code/mpfr/mpfr-c/MPFR.c
@@ -118,6 +118,11 @@ static void MPFR_Lib_mpn_ZERO(uint64_t *b, uint32_t l)
   }
 }
 
+static int32_t MPFR_Lib_mpfr_RET(int32_t t)
+{
+  return t;
+}
+
 static void MPFR_Lib_mpfr_setmax_rec(MPFR_Lib_mpfr_struct *x, uint32_t i)
 {
   uint64_t *mant = x->mpfr_d;
@@ -138,14 +143,14 @@ static void MPFR_Lib_mpfr_setmax_rec(MPFR_Lib_mpfr_struct *x, uint32_t i)
 
 static void MPFR_Lib_mpfr_setmax(MPFR_Lib_mpfr_struct *x)
 {
-  MPFR_Lib_mpfr_struct uu___72_131209 = x[0U];
+  MPFR_Lib_mpfr_struct uu___62_131220 = x[0U];
   x[0U] =
     (
       (MPFR_Lib_mpfr_struct){
-        .mpfr_prec = uu___72_131209.mpfr_prec,
-        .mpfr_sign = uu___72_131209.mpfr_sign,
+        .mpfr_prec = uu___62_131220.mpfr_prec,
+        .mpfr_sign = uu___62_131220.mpfr_sign,
         .mpfr_exp = MPFR_Lib_mpfr_EMAX,
-        .mpfr_d = uu___72_131209.mpfr_d
+        .mpfr_d = uu___62_131220.mpfr_d
       }
     );
   MPFR_Lib_mpfr_struct f = x[0U];
@@ -154,14 +159,14 @@ static void MPFR_Lib_mpfr_setmax(MPFR_Lib_mpfr_struct *x)
 
 static void MPFR_Lib_mpfr_setmin(MPFR_Lib_mpfr_struct *x)
 {
-  MPFR_Lib_mpfr_struct uu___72_131420 = x[0U];
+  MPFR_Lib_mpfr_struct uu___62_131431 = x[0U];
   x[0U] =
     (
       (MPFR_Lib_mpfr_struct){
-        .mpfr_prec = uu___72_131420.mpfr_prec,
-        .mpfr_sign = uu___72_131420.mpfr_sign,
+        .mpfr_prec = uu___62_131431.mpfr_prec,
+        .mpfr_sign = uu___62_131431.mpfr_sign,
         .mpfr_exp = MPFR_Lib_mpfr_EMIN,
-        .mpfr_d = uu___72_131420.mpfr_d
+        .mpfr_d = uu___62_131431.mpfr_d
       }
     );
   MPFR_Lib_mpfr_struct f = x[0U];
@@ -178,14 +183,14 @@ MPFR_Exceptions_mpfr_overflow(
   int32_t sign
 )
 {
-  MPFR_Lib_mpfr_struct uu___73_80 = x[0U];
+  MPFR_Lib_mpfr_struct uu___63_80 = x[0U];
   x[0U] =
     (
       (MPFR_Lib_mpfr_struct){
-        .mpfr_prec = uu___73_80.mpfr_prec,
+        .mpfr_prec = uu___63_80.mpfr_prec,
         .mpfr_sign = sign,
-        .mpfr_exp = uu___73_80.mpfr_exp,
-        .mpfr_d = uu___73_80.mpfr_d
+        .mpfr_exp = uu___63_80.mpfr_exp,
+        .mpfr_d = uu___63_80.mpfr_d
       }
     );
   if (MPFR_RoundingMode_mpfr_IS_LIKE_RNDZ(rnd_mode, sign < (int32_t)0))
@@ -198,14 +203,14 @@ MPFR_Exceptions_mpfr_overflow(
   }
   else
   {
-    MPFR_Lib_mpfr_struct uu___72_167 = x[0U];
+    MPFR_Lib_mpfr_struct uu___62_167 = x[0U];
     x[0U] =
       (
         (MPFR_Lib_mpfr_struct){
-          .mpfr_prec = uu___72_167.mpfr_prec,
-          .mpfr_sign = uu___72_167.mpfr_sign,
+          .mpfr_prec = uu___62_167.mpfr_prec,
+          .mpfr_sign = uu___62_167.mpfr_sign,
           .mpfr_exp = (int32_t)-0x80000000 + (int32_t)3,
-          .mpfr_d = uu___72_167.mpfr_d
+          .mpfr_d = uu___62_167.mpfr_d
         }
       );
     return sign;
@@ -219,26 +224,26 @@ MPFR_Exceptions_mpfr_underflow(
   int32_t sign
 )
 {
-  MPFR_Lib_mpfr_struct uu___73_284 = x[0U];
+  MPFR_Lib_mpfr_struct uu___63_284 = x[0U];
   x[0U] =
     (
       (MPFR_Lib_mpfr_struct){
-        .mpfr_prec = uu___73_284.mpfr_prec,
+        .mpfr_prec = uu___63_284.mpfr_prec,
         .mpfr_sign = sign,
-        .mpfr_exp = uu___73_284.mpfr_exp,
-        .mpfr_d = uu___73_284.mpfr_d
+        .mpfr_exp = uu___63_284.mpfr_exp,
+        .mpfr_d = uu___63_284.mpfr_d
       }
     );
   if (MPFR_RoundingMode_mpfr_IS_LIKE_RNDZ(rnd_mode, sign < (int32_t)0))
   {
-    MPFR_Lib_mpfr_struct uu___72_339 = x[0U];
+    MPFR_Lib_mpfr_struct uu___62_339 = x[0U];
     x[0U] =
       (
         (MPFR_Lib_mpfr_struct){
-          .mpfr_prec = uu___72_339.mpfr_prec,
-          .mpfr_sign = uu___72_339.mpfr_sign,
+          .mpfr_prec = uu___62_339.mpfr_prec,
+          .mpfr_sign = uu___62_339.mpfr_sign,
           .mpfr_exp = (int32_t)-0x80000000 + (int32_t)1,
-          .mpfr_d = uu___72_339.mpfr_d
+          .mpfr_d = uu___62_339.mpfr_d
         }
       );
     if (sign == (int32_t)1)
@@ -479,18 +484,18 @@ MPFR_Add1sp1_mpfr_add1sp1(
   {
     uint64_t *ap = a->mpfr_d;
     uint64_t a01 = ap[0U];
-    MPFR_Lib_mpfr_struct uu___72_3461 = a[0U];
+    MPFR_Lib_mpfr_struct uu___62_3483 = a[0U];
     a[0U] =
       (
         (MPFR_Lib_mpfr_struct){
-          .mpfr_prec = uu___72_3461.mpfr_prec,
-          .mpfr_sign = uu___72_3461.mpfr_sign,
+          .mpfr_prec = uu___62_3483.mpfr_prec,
+          .mpfr_sign = uu___62_3483.mpfr_sign,
           .mpfr_exp = st.bx,
-          .mpfr_d = uu___72_3461.mpfr_d
+          .mpfr_d = uu___62_3483.mpfr_d
         }
       );
     if (st.rb == (uint64_t)0U && st.sb == (uint64_t)0U)
-      return (int32_t)0;
+      return MPFR_Lib_mpfr_RET((int32_t)0);
     else if (MPFR_RoundingMode_uu___is_MPFR_RNDN(rnd_mode))
       if
       (
@@ -498,10 +503,14 @@ MPFR_Add1sp1_mpfr_add1sp1(
         == (uint64_t)0U
         || (st.sb == (uint64_t)0U && (a01 & (uint64_t)1U << st.sh) == (uint64_t)0U)
       )
+      {
+        int32_t ite;
         if (a->mpfr_sign == (int32_t)1)
-          return (int32_t)-1;
+          ite = (int32_t)-1;
         else
-          return (int32_t)1;
+          ite = (int32_t)1;
+        return MPFR_Lib_mpfr_RET(ite);
+      }
       else
       {
         uint64_t *ap1 = a->mpfr_d;
@@ -511,32 +520,36 @@ MPFR_Add1sp1_mpfr_add1sp1(
           ap1[0U] = (uint64_t)0x8000000000000000U;
           if (st.bx + (int32_t)1 <= MPFR_Lib_mpfr_EMAX)
           {
-            MPFR_Lib_mpfr_struct uu___72_3556 = a[0U];
+            MPFR_Lib_mpfr_struct uu___62_3579 = a[0U];
             a[0U] =
               (
                 (MPFR_Lib_mpfr_struct){
-                  .mpfr_prec = uu___72_3556.mpfr_prec,
-                  .mpfr_sign = uu___72_3556.mpfr_sign,
+                  .mpfr_prec = uu___62_3579.mpfr_prec,
+                  .mpfr_sign = uu___62_3579.mpfr_sign,
                   .mpfr_exp = st.bx + (int32_t)1,
-                  .mpfr_d = uu___72_3556.mpfr_d
+                  .mpfr_d = uu___62_3579.mpfr_d
                 }
               );
-            return a->mpfr_sign;
+            return MPFR_Lib_mpfr_RET(a->mpfr_sign);
           }
           else
           {
             int32_t t = MPFR_Exceptions_mpfr_overflow(a, rnd_mode, a->mpfr_sign);
-            return t;
+            return MPFR_Lib_mpfr_RET(t);
           }
         }
         else
-          return a->mpfr_sign;
+          return MPFR_Lib_mpfr_RET(a->mpfr_sign);
       }
     else if (MPFR_RoundingMode_mpfr_IS_LIKE_RNDZ(rnd_mode, a->mpfr_sign < (int32_t)0))
+    {
+      int32_t ite;
       if (a->mpfr_sign == (int32_t)1)
-        return (int32_t)-1;
+        ite = (int32_t)-1;
       else
-        return (int32_t)1;
+        ite = (int32_t)1;
+      return MPFR_Lib_mpfr_RET(ite);
+    }
     else
     {
       uint64_t *ap1 = a->mpfr_d;
@@ -546,26 +559,26 @@ MPFR_Add1sp1_mpfr_add1sp1(
         ap1[0U] = (uint64_t)0x8000000000000000U;
         if (st.bx + (int32_t)1 <= MPFR_Lib_mpfr_EMAX)
         {
-          MPFR_Lib_mpfr_struct uu___72_3760 = a[0U];
+          MPFR_Lib_mpfr_struct uu___62_3786 = a[0U];
           a[0U] =
             (
               (MPFR_Lib_mpfr_struct){
-                .mpfr_prec = uu___72_3760.mpfr_prec,
-                .mpfr_sign = uu___72_3760.mpfr_sign,
+                .mpfr_prec = uu___62_3786.mpfr_prec,
+                .mpfr_sign = uu___62_3786.mpfr_sign,
                 .mpfr_exp = st.bx + (int32_t)1,
-                .mpfr_d = uu___72_3760.mpfr_d
+                .mpfr_d = uu___62_3786.mpfr_d
               }
             );
-          return a->mpfr_sign;
+          return MPFR_Lib_mpfr_RET(a->mpfr_sign);
         }
         else
         {
           int32_t t = MPFR_Exceptions_mpfr_overflow(a, rnd_mode, a->mpfr_sign);
-          return t;
+          return MPFR_Lib_mpfr_RET(t);
         }
       }
       else
-        return a->mpfr_sign;
+        return MPFR_Lib_mpfr_RET(a->mpfr_sign);
     }
   }
 }
@@ -635,14 +648,14 @@ MPFR_Mul_1_mpfr_mul_1(
   uint64_t rb = a01 & (uint64_t)1U << (sh - (uint32_t)1U);
   uint64_t sb2 = sb1 | ((a01 & mask) ^ rb);
   ap[0U] = a01 & ~mask;
-  MPFR_Lib_mpfr_struct uu___73_2684 = a[0U];
+  MPFR_Lib_mpfr_struct uu___63_2684 = a[0U];
   a[0U] =
     (
       (MPFR_Lib_mpfr_struct){
-        .mpfr_prec = uu___73_2684.mpfr_prec,
+        .mpfr_prec = uu___63_2684.mpfr_prec,
         .mpfr_sign = b->mpfr_sign * c->mpfr_sign,
-        .mpfr_exp = uu___73_2684.mpfr_exp,
-        .mpfr_d = uu___73_2684.mpfr_d
+        .mpfr_exp = uu___63_2684.mpfr_exp,
+        .mpfr_d = uu___63_2684.mpfr_d
       }
     );
   uint64_t *ap1 = a->mpfr_d;
@@ -664,14 +677,14 @@ MPFR_Mul_1_mpfr_mul_1(
     {
       uint64_t *ap2 = a->mpfr_d;
       uint64_t a03 = ap2[0U];
-      MPFR_Lib_mpfr_struct uu___72_2835 = a[0U];
+      MPFR_Lib_mpfr_struct uu___62_2835 = a[0U];
       a[0U] =
         (
           (MPFR_Lib_mpfr_struct){
-            .mpfr_prec = uu___72_2835.mpfr_prec,
-            .mpfr_sign = uu___72_2835.mpfr_sign,
+            .mpfr_prec = uu___62_2835.mpfr_prec,
+            .mpfr_sign = uu___62_2835.mpfr_sign,
             .mpfr_exp = ax1,
-            .mpfr_d = uu___72_2835.mpfr_d
+            .mpfr_d = uu___62_2835.mpfr_d
           }
         );
       if (rb == (uint64_t)0U && sb2 == (uint64_t)0U)
@@ -694,14 +707,14 @@ MPFR_Mul_1_mpfr_mul_1(
               return MPFR_Exceptions_mpfr_overflow(a, rnd_mode, a->mpfr_sign);
             else
             {
-              MPFR_Lib_mpfr_struct uu___72_2974 = a[0U];
+              MPFR_Lib_mpfr_struct uu___62_2974 = a[0U];
               a[0U] =
                 (
                   (MPFR_Lib_mpfr_struct){
-                    .mpfr_prec = uu___72_2974.mpfr_prec,
-                    .mpfr_sign = uu___72_2974.mpfr_sign,
+                    .mpfr_prec = uu___62_2974.mpfr_prec,
+                    .mpfr_sign = uu___62_2974.mpfr_sign,
                     .mpfr_exp = ax1 + (int32_t)1,
-                    .mpfr_d = uu___72_2974.mpfr_d
+                    .mpfr_d = uu___62_2974.mpfr_d
                   }
                 );
               return a->mpfr_sign;
@@ -726,14 +739,14 @@ MPFR_Mul_1_mpfr_mul_1(
             return MPFR_Exceptions_mpfr_overflow(a, rnd_mode, a->mpfr_sign);
           else
           {
-            MPFR_Lib_mpfr_struct uu___72_3161 = a[0U];
+            MPFR_Lib_mpfr_struct uu___62_3161 = a[0U];
             a[0U] =
               (
                 (MPFR_Lib_mpfr_struct){
-                  .mpfr_prec = uu___72_3161.mpfr_prec,
-                  .mpfr_sign = uu___72_3161.mpfr_sign,
+                  .mpfr_prec = uu___62_3161.mpfr_prec,
+                  .mpfr_sign = uu___62_3161.mpfr_sign,
                   .mpfr_exp = ax1 + (int32_t)1,
-                  .mpfr_d = uu___72_3161.mpfr_d
+                  .mpfr_d = uu___62_3161.mpfr_d
                 }
               );
             return a->mpfr_sign;
@@ -759,14 +772,14 @@ MPFR_Mul_1_mpfr_mul_1(
   {
     uint64_t *ap2 = a->mpfr_d;
     uint64_t a03 = ap2[0U];
-    MPFR_Lib_mpfr_struct uu___72_3344 = a[0U];
+    MPFR_Lib_mpfr_struct uu___62_3344 = a[0U];
     a[0U] =
       (
         (MPFR_Lib_mpfr_struct){
-          .mpfr_prec = uu___72_3344.mpfr_prec,
-          .mpfr_sign = uu___72_3344.mpfr_sign,
+          .mpfr_prec = uu___62_3344.mpfr_prec,
+          .mpfr_sign = uu___62_3344.mpfr_sign,
           .mpfr_exp = ax1,
-          .mpfr_d = uu___72_3344.mpfr_d
+          .mpfr_d = uu___62_3344.mpfr_d
         }
       );
     if (rb == (uint64_t)0U && sb2 == (uint64_t)0U)
@@ -788,14 +801,14 @@ MPFR_Mul_1_mpfr_mul_1(
             return MPFR_Exceptions_mpfr_overflow(a, rnd_mode, a->mpfr_sign);
           else
           {
-            MPFR_Lib_mpfr_struct uu___72_3483 = a[0U];
+            MPFR_Lib_mpfr_struct uu___62_3483 = a[0U];
             a[0U] =
               (
                 (MPFR_Lib_mpfr_struct){
-                  .mpfr_prec = uu___72_3483.mpfr_prec,
-                  .mpfr_sign = uu___72_3483.mpfr_sign,
+                  .mpfr_prec = uu___62_3483.mpfr_prec,
+                  .mpfr_sign = uu___62_3483.mpfr_sign,
                   .mpfr_exp = ax1 + (int32_t)1,
-                  .mpfr_d = uu___72_3483.mpfr_d
+                  .mpfr_d = uu___62_3483.mpfr_d
                 }
               );
             return a->mpfr_sign;
@@ -820,14 +833,14 @@ MPFR_Mul_1_mpfr_mul_1(
           return MPFR_Exceptions_mpfr_overflow(a, rnd_mode, a->mpfr_sign);
         else
         {
-          MPFR_Lib_mpfr_struct uu___72_3670 = a[0U];
+          MPFR_Lib_mpfr_struct uu___62_3670 = a[0U];
           a[0U] =
             (
               (MPFR_Lib_mpfr_struct){
-                .mpfr_prec = uu___72_3670.mpfr_prec,
-                .mpfr_sign = uu___72_3670.mpfr_sign,
+                .mpfr_prec = uu___62_3670.mpfr_prec,
+                .mpfr_sign = uu___62_3670.mpfr_sign,
                 .mpfr_exp = ax1 + (int32_t)1,
-                .mpfr_d = uu___72_3670.mpfr_d
+                .mpfr_d = uu___62_3670.mpfr_d
               }
             );
           return a->mpfr_sign;
